theories/ftlr/Get.v
@@ -31,7 +31,7 @@ Section fundamental.
     ftlr_instr W regs p p' g b e a w ins ρ P.
   Proof.
     intros Hinstr Hp Hsome i Hbae Hfp HO Hpers Hpwl Hregion Hnotrevoked Hnotfrozen Hi.
-    iIntros "#IH #Hinv_interp #Hreg #Hinva #Hrcond #Hwcond #HmonoV #Hmono Hw Hsts Hown".
+    iIntros "#IH #Hinv_interp #Hreg #Hinva #Hrcond #Hwcond #Hmono #HmonoV Hw Hsts Hown".
     iIntros "Hr Hstate Ha HPC Hmap".
     rewrite <- Hi in Hinstr; clear Hi.
     iInsert "Hmap" PC.
@@ -48,7 +48,7 @@ Section fundamental.
       iApply wp_pure_step_later; auto. iNext; iIntros "_".
       assert (dst <> PC) as HdstPC by (intros ->; simplify_map_eq).
       simplify_map_eq.
-      iDestruct (region_close with "[$Hstate $Hr $Ha $Hmono Hw]") as "Hr"; eauto.
+      iDestruct (region_close with "[$Hstate $Hr $Ha $HmonoV Hw]") as "Hr"; eauto.
       { destruct ρ;auto;[|specialize (Hnotfrozen g)];contradiction. }
 
       iApply ("IH" $! _ (<[dst := _]> (<[PC := _]> regs))
