theories/ftlr/Subseg.v
@@ -45,7 +45,7 @@ Section fundamental.
     ftlr_instr W regs p p' g b e a w (Subseg dst r1 r2) ρ P.
   Proof.
     intros Hp Hsome i Hbae Hfp HO Hpers Hpwl Hregion Hnotrevoked Hnotfrozen Hi.
-    iIntros "#IH #Hinv_interp #Hreg #Hinva #Hrcond #Hwcond #HmonoV #Hmono Hw Hsts Hown".
+    iIntros "#IH #Hinv_interp #Hreg #Hinva #Hrcond #Hwcond #Hmono #HmonoV Hw Hsts Hown".
     iIntros "Hr Hstate Ha HPC Hmap".
     iInsert "Hmap" PC.
     iApply (wp_Subseg with "[$Ha $Hmap]"); eauto.
@@ -65,7 +65,7 @@ Section fundamental.
 
       iApply wp_pure_step_later; auto.
       iNext ; iIntros "_".
-      iDestruct (region_close with "[$Hstate $Hr $Ha $Hmono Hw]") as "Hr"; eauto.
+      iDestruct (region_close with "[$Hstate $Hr $Ha $HmonoV Hw]") as "Hr"; eauto.
       { destruct ρ;auto;[|ospecialize (Hnotfrozen _)];contradiction. }
       simplify_map_eq; map_simpl "Hmap".
 
@@ -103,7 +103,7 @@ Section fundamental.
 
       iApply wp_pure_step_later; auto.
       iNext ; iIntros "_".
-      iDestruct (region_close with "[$Hstate $Hr $Ha $Hmono Hw]") as "Hr"; eauto.
+      iDestruct (region_close with "[$Hstate $Hr $Ha $HmonoV Hw]") as "Hr"; eauto.
       { destruct ρ;auto;[|ospecialize (Hnotfrozen _)];contradiction. }
       simplify_map_eq; map_simpl "Hmap".
 
