theories/ftlr/UnSeal.v
@@ -55,7 +55,7 @@ Section fundamental.
     ftlr_instr W regs p p' g b e a w (UnSeal dst r1 r2) ρ P.
   Proof.
     intros Hp Hsome i Hbae Hfp HO Hpers Hpwl Hregion Hnotrevoked Hnotfrozen Hi.
-    iIntros "#IH #Hinv_interp #Hreg #Hinva #Hrcond #Hwcond #HmonoV #Hmono Hw Hsts Hown".
+    iIntros "#IH #Hinv_interp #Hreg #Hinva #Hrcond #Hwcond #Hmono #HmonoV Hw Hsts Hown".
     iIntros "Hr Hstate Ha HPC Hmap".
     iInsert "Hmap" PC.
     iApply (wp_UnSeal with "[$Ha $Hmap]"); eauto.
@@ -85,7 +85,7 @@ Section fundamental.
     iDestruct (unsealing_preserves_interp with "HVsd HVsr") as "HVsb"; auto.
 
     iApply wp_pure_step_later; auto; iNext; iIntros "_".
-    iDestruct (region_close with "[$Hstate $Hr $Ha $Hmono Hw]") as "Hr"; eauto.
+    iDestruct (region_close with "[$Hstate $Hr $Ha $HmonoV Hw]") as "Hr"; eauto.
     { destruct ρ;auto;[|ospecialize (Hnotfrozen _)];contradiction. }
 
     (* If PC=dst and perm of unsealed cap = E -> error! *)
