theories/ftlr/ftlr_base.v
@@ -60,12 +60,10 @@ Section fundamental.
     -∗ □ (if decide (writeAllowed_in_r_a (<[PC:=(WCap p g b e a)]> regs) a)
           then ▷ wcond P interp
           else emp)
+    -∗ monoReq W a p' P
     -∗ (▷ (if decide (ρ = Temporary /\ pwl p' = true)
            then future_pub_mono (safeC P) w
            else future_priv_mono (safeC P) w))
-    -∗ (▷ (if decide (ρ = Temporary /\ pwl p' = true)
-           then mono_pub (safeC P)
-           else mono_priv (safeC P) p'))
     -∗ ▷ P W w
     -∗ sts_full_world W
     -∗ na_own logrel_nais ⊤
